#数学
# Polynomial equation
## Cubic equation in one element
### An example
$$
\begin{array}{c}
a+b+c=1\\
a^{2} +b^{2} +c^{2} =2\\
a^{3} +b^{3} +c^{3} =3\\
\ \\
ab+bc+ac=-\frac{1}{2}\\
x^{3} -x^{2} -\frac{1}{2}x -abc =0 \\
a^{3} -a^{2} -\frac{1}{2}a -abc =0 \\
b^{3} -b^{2} -\frac{1}{2}b -abc =0 \\
c^{3} -c^{2} -\frac{1}{2}c -abc =0 \\
(a^3+b^3+c^3) -(a^2+b^2+c^2) -\frac{1}{2}(a+b+c) -3abc =0\\
abc=\frac{1}{6}\\
x^{3} -x^{2} -\frac{1}{2}x -\frac{1}{6} =0 \\
\end{array}
$$
let $\displaystyle f_{n} =a^{n} +b^{n} +c^{n}$，we get $\displaystyle f_{n} =f_{n-1} +\frac{1}{2} f_{n-2} +\frac{1}{6} f_{n-3}$，$\displaystyle n >3$
# Inequality

## Simple algebraic inequalities

### Average inequality

#### Broad form

see in [[初等分析#加权平均不等式|加权平均不等式]]

#### Proofs based on mathematical induction

The following methods are all based on [[Mathematical Logic#mathematical induction|mathematical induction]]

## Analytical inequalities
see in [[初等分析#分析不等式|分析不等式]]

## Geometric inequalities
